Mapping of names from verilog to netlist

vvequiv/VerilogToNetlist.v
@@ -2,28 +2,66 @@ Require Verilog.
 Require Netlist.
 Require Import ZArith.
 Require Import BinIntDef.
+Require Import String.
+Require Import FSets.
+Require Import FMaps.
 
 Require Import List.
 Import ListNotations.
 
 From ExtLib Require Import Structures.Monads.
+From ExtLib Require Import Structures.MonadState.
 From ExtLib Require Import Structures.Functor.
 From ExtLib Require Import Structures.Traversable.
 From ExtLib Require Import Data.Monads.StateMonad.
+From ExtLib Require Import Data.Monads.EitherMonad.
 From ExtLib Require Import Data.List.
 Import MonadNotation.
+Open Scope monad_scope.
+Require Import Program.
 
-Definition transf := state Z.
+Module StrMap := FMapList.Make(String_as_OT).
 
-Definition fresh : transf Z := mkState (fun n => (n, Z.succ n)).
+Record transf_state :=
+  TransfState
+    { nextName : N;
+      nameMap : StrMap.t N
+    }.
 
-Definition transfer_type (type : Verilog.vtype) : transf Netlist.nltype :=
-  match type with
-  | Verilog.Logic hi lo => ret (Netlist.Logic (hi - lo + 1))
-  end
+Definition transf : Type -> Type := stateT transf_state (sum string).
+
+Instance Monad_transf : Monad transf := Monad_stateT transf_state (Monad_either string).
+
+Definition fresh : transf N :=
+  s <- get ;;
+  let s' := {| nextName := N.succ (nextName s) ; nameMap := nameMap s |} in
+  put s' ;;
+  ret (nextName s)
 .
 
-Open Scope monad_scope.
+Definition map_name (name : string) : transf N :=
+  st <- get ;;
+  match StrMap.find name (nameMap st) with
+  | Some n => ret n
+  | None =>
+      n <- fresh ;;
+      put {|
+          nextName := (nextName st) ;
+          nameMap := StrMap.add name n (nameMap st)
+        |} ;;
+      ret n
+  end.
+
+
+Definition transfer_type (type : Verilog.vtype) : transf Netlist.nltype :=
+  (* Probably wrong but good enough for now*)
+  match type with
+  | Verilog.Logic N0 N0 => ret (Netlist.Logic 1)
+  | Verilog.Logic (Npos n) N0 => ret (Netlist.Logic (n + 1))
+  | Verilog.Logic N0 (Npos n) => ret (Netlist.Logic (n + 1))
+  | Verilog.Logic (Npos n1) (Npos n2) => ret (Netlist.Logic (n1 - n2 + 1))
+  end
+.
 
 Definition transfer_variables (vars : list Verilog.variable) : transf (list Netlist.variable) :=
   mapT (fun v =>
